<?xml version="1.0"?>

<!-- $Id: location,v 1.1 2004/10/13 15:44:03 icm02r Exp $ -->

<!DOCTYPE owl [
  <!ENTITY rdf		"http://www.w3.org/1999/02/22-rdf-syntax-ns#">
  <!ENTITY rdfs		"http://www.w3.org/2000/01/rdf-schema#">
  <!ENTITY xsd		"http://www.w3.org/2001/XMLSchema#"> 
  <!ENTITY owl		"http://www.w3.org/2002/07/owl#">
  <!ENTITY dc		"http://purl.org/dc/elements/1.1/">
  <!ENTITY dct		"http://purl.org/dc/terms/">
  <!ENTITY portal	"http://www.aktors.org/ontology/portal#">   
  <!ENTITY extension	"http://www.aktors.org/ontology/extension#">
  <!ENTITY ome		"http://contextus.net/ontology/ontomedia/core/expression#">  
  <!ENTITY base		"http://signage.ecs.soton.ac.uk/ontologies/location#">  
]>

<rdf:RDF xmlns:rdf="&rdf;"
         xmlns:rdfs="&rdfs;"
         xmlns:xsd="&xsd;"
         xmlns:owl="&owl;"
         xmlns:dc="&dc;"
         xmlns:dct="&dct;"
         xmlns:ome="&ome;"
         xmlns:portal="&portal;"
         xmlns:base="&base;">

  <owl:Ontology rdf:about="&base;">
    <rdfs:label>Building Ontology</rdfs:label>
    <dc:title xml:lang="en">Building Ontology</dc:title>
    <dc:description xml:lang="en">The Building Ontology has been designed to describe the structure, contents and occupants of a building, in order support a number of pervasive computing applications.</dc:description>
    <dc:creator>Ian Millard (icm02r@ecs.soton.ac.uk)</dc:creator>
    <dct:created>2004-08-05</dct:created>
    <owl:versionInfo>0.6</owl:versionInfo>
    <owl:imports rdf:resource="http://www.aktors.org/ontology/portal" />
    <owl:imports rdf:resource="http://www.aktors.org/ontology/extension" />
  </owl:Ontology>



  <!-- Abstract space, and associated properties -->

  <owl:Class rdf:ID="Abstract-Space">
    <rdfs:label>Abstract Space</rdfs:label>
    <rdfs:subClassOf rdf:resource="&ome;Entity"/>
    <rdfs:comment>This is a high-level abstraction of any space, area, or location</rdfs:comment>
    <owl:equivalentClass rdf:resource="&portal;Location"/>
  </owl:Class>

  <owl:ObjectProperty rdf:ID="is-located-in">
    <rdf:type rdf:resource="&owl;TransitiveProperty"/>
    <rdfs:label>is located in</rdfs:label>
    <rdfs:comment>This property is to be used to describe anything which is located in an Abstract-Space (quite possibly another Abstract Space)</rdfs:comment>
    <rdfs:domain rdf:resource="&owl;Thing" />
    <rdfs:range rdf:resource="#Abstract-Space" />
  </owl:ObjectProperty>

  <owl:ObjectProperty rdf:ID="is-located-at">
    <rdf:type rdf:resource="&owl;TransitiveProperty"/>
    <rdfs:label>is located at</rdfs:label>
    <rdfs:comment>This property is to be used to describe anything which is located at a Coordinate-Position</rdfs:comment>
    <rdfs:domain rdf:resource="&owl;Thing" />
    <rdfs:range rdf:resource="#Coordinate-Position" />
  </owl:ObjectProperty>

  <!-- owl:ObjectProperty rdf:ID="is-part-of">
    <rdfs:label>is part of</rdfs:label>
    <rdfs:comment>This property is to be used to describe an Abstract-Space which forms part of another</rdfs:comment>
    <rdfs:domain rdf:resource="#Abstract-Space" />
    <rdfs:range rdf:resource="#Abstract-Space" />
  </owl:ObjectProperty -->

  <owl:ObjectProperty rdf:ID="is-owned-by">
    <rdfs:label>is owned by</rdfs:label>
    <rdfs:comment>This property is to be used to describe the owning agent (organisation or person) of the Abstract-Space</rdfs:comment>
    <rdfs:domain rdf:resource="#Abstract-Space" />
    <rdfs:range rdf:resource="&portal;Generic-Agent" />
  </owl:ObjectProperty>    

  <owl:ObjectProperty rdf:ID="has-usual-occupant">
    <rdfs:label>has usual occupant</rdfs:label>
    <rdfs:comment>This property is to be used to describe the usual occupant of an Abstract-Space</rdfs:comment>
    <rdfs:domain rdf:resource="#Abstract-Space" />
    <rdfs:range rdf:resource="&portal;Person" />
  </owl:ObjectProperty>

  <owl:ObjectProperty rdf:ID="is-visible-from">
    <rdfs:label>is visible from</rdfs:label>
    <rdfs:comment>This property can be used to describe the fact that the thing in question is visible from the specified location</rdfs:comment>
    <rdfs:domain rdf:resource="&owl;Thing" />
    <rdfs:range  rdf:resource="#Abstract-Space" />
    <owl:inverseOf rdf:resource="#permits-viewing-of" />
  </owl:ObjectProperty>

  <owl:ObjectProperty rdf:ID="permits-viewing-of">
    <rdfs:label>permits viewing of</rdfs:label>
    <rdfs:comment>This property can be used to describe the fact that when located at the abstract space in question, the specified thing can be viewed</rdfs:comment>
    <rdfs:domain rdf:resource="#Abstract-Space" />
    <rdfs:range  rdf:resource="&owl;Thing" />
    <owl:inverseOf rdf:resource="#permits-viewing-of" />
  </owl:ObjectProperty>

  <owl:ObjectProperty rdf:ID="adjacent-to">
    <rdfs:label>adjacent to</rdfs:label>
    <rdfs:comment>This property indicates that one Abstract Space is adjacent to another</rdfs:comment>
    <rdfs:domain rdf:resource="#Abstract-Space" />
    <rdfs:range  rdf:resource="#Abstract-Space" />
  </owl:ObjectProperty> 

  <owl:ObjectProperty rdf:ID="adjacent-to-on-north-side">
    <rdfs:label>adjacent to on north side</rdfs:label>
    <rdfs:comment>This property is to be used to describe an adjacent Abstract Space which is to the North</rdfs:comment>
    <rdfs:subPropertyOf rdf:resource="#adjacent-to" />
    <owl:inverseOf rdf:resource="#adjacent-to-on-south-side" />
  </owl:ObjectProperty>

  <owl:ObjectProperty rdf:ID="adjacent-to-on-south-side">
    <rdfs:label>adjacent to on south side</rdfs:label>
    <rdfs:comment>This property is to be used to describe an adjacent Abstract Space which is to the South</rdfs:comment>
    <owl:inverseOf rdf:resource="#adjacent-to-on-north-side" />
    <rdfs:subPropertyOf rdf:resource="#adjacent-to" />
  </owl:ObjectProperty>

  <owl:ObjectProperty rdf:ID="adjacent-to-on-east-side">
    <rdfs:label>adjacent to on east side</rdfs:label>
    <rdfs:comment>This property is to be used to describe an adjacent Abstract Space which is to the East</rdfs:comment>
    <rdfs:subPropertyOf rdf:resource="#adjacent-to" />
    <owl:inverseOf rdf:resource="#adjacent-to-on-west-side" />
  </owl:ObjectProperty>

  <owl:ObjectProperty rdf:ID="adjacent-to-on-west-side">
    <rdfs:label>adjacent to on west side</rdfs:label>
    <rdfs:comment>This property is to be used to describe an adjacent Abstract Space which is to the West</rdfs:comment>
    <rdfs:subPropertyOf rdf:resource="#adjacent-to" />
    <owl:inverseOf rdf:resource="#adjacent-to-on-east-side" />
  </owl:ObjectProperty>

  <owl:ObjectProperty rdf:ID="has-bounding-coordinates">
    <rdfs:label>has-bounding-coordinates</rdfs:label>
    <rdfs:comment>A sequence of bounding Coordinate-Position resources which form the bounds of this Abstract-Space</rdfs:comment>
    <rdfs:domain rdf:resource="#Abstract-Space" />
    <rdfs:range rdf:resource="#Sequence-Of-Coordinates" />
  </owl:ObjectProperty>

  <owl:Class rdf:ID="Sequence-Of-Coordinates">
    <rdfs:subClassOf rdf:resource="&rdf;Seq"/>
  </owl:Class>

  <owl:ObjectProperty rdf:ID="has-origin-coordinate">
    <rdfs:label>has-origin-coordinate</rdfs:label>
    <rdfs:comment>The Origin Coordinate of this Abstract-Space</rdfs:comment>
    <rdfs:domain rdf:resource="#Abstract-Space" />
    <rdfs:range rdf:resource="#Coordinate-Position" />
  </owl:ObjectProperty>

  <owl:Class rdf:ID="Abstract-Space-With-Origin">
    <rdfs:label>Abstract-Space-With-Origin</rdfs:label>
    <rdfs:comment>An abstract space which has a origin-coordinate</rdfs:comment>
    <rdfs:subClassOf rdf:resource="#Abstract-Space"/>
    <rdfs:subClassOf>
      <owl:Restriction>
        <owl:onProperty rdf:resource="#has-origin-coordinate"/>
        <owl:cardinality rdf:datatype="&xsd;integer">1</owl:cardinality>
      </owl:Restriction>
    </rdfs:subClassOf>
  </owl:Class>



  <!-- Open space -->

  <owl:Class rdf:ID="Open-Space">
    <rdfs:label>Open Space</rdfs:label>
    <rdfs:comment>This is a high-level abstraction of any open (un-bounded) space, offering unrestricted movement in and out of the space</rdfs:comment>
    <rdfs:subClassOf rdf:resource="#Abstract-Space" />
  </owl:Class>



  <!-- Enclosed space, and associated properties -->

  <owl:Class rdf:ID="Enclosed-Space">
    <rdfs:label>Enclosed Space</rdfs:label>
    <rdfs:comment>This is a high-level abstraction of any enclosed or bounded space (such as a building or room) which constrians movement from one space to another</rdfs:comment>
    <rdfs:subClassOf rdf:resource="#Abstract-Space" />
  </owl:Class>

  <owl:ObjectProperty rdf:ID="permits-access-to">
    <rdfs:label>permits access to</rdfs:label>
    <rdfs:comment>This property is to be used to describe a connection (such as a door) which permits access between two Enclosed-Spaces</rdfs:comment>
    <rdfs:domain rdf:resource="#Enclosed-Space" />
    <rdfs:range rdf:resource="#Abstract-Space" />
  </owl:ObjectProperty>



  <!-- A building -->

  <owl:Class rdf:ID="Building">
    <rdfs:label>Building</rdfs:label>
    <rdfs:comment>This class is used to represent a Building</rdfs:comment>
    <rdfs:subClassOf rdf:resource="#Enclosed-Space" />
  </owl:Class>

  <owl:ObjectProperty rdf:ID="has-postal-address">
    <rdfs:label>has postal address</rdfs:label>
    <rdfs:comment>This property denotes that a Building is located at a particular Postal-Address</rdfs:comment>
    <rdfs:domain rdf:resource="#Building" />
    <rdfs:range  rdf:resource="&portal;Postal-Address" />
  </owl:ObjectProperty>



  <!-- A floor in a building -->

  <owl:Class rdf:ID="Floor">
    <rdfs:label>Floor</rdfs:label>
    <rdfs:comment>This class is used to represent a Floor in a Building</rdfs:comment>
    <rdfs:subClassOf rdf:resource="#Enclosed-Space" />
    <rdfs:subClassOf>
      <owl:Restriction> 
        <owl:onProperty rdf:resource="#is-part-of" />
        <owl:allValuesFrom rdf:resource="#Building" />
      </owl:Restriction>
    </rdfs:subClassOf>
  </owl:Class>



  <!-- A Room on a Floor of a Building -->

  <owl:Class rdf:ID="Room">
    <rdfs:label>Room</rdfs:label>
    <rdfs:comment>This class is used to represent a Room on a Floor in a Building</rdfs:comment>
    <rdfs:subClassOf rdf:resource="#Enclosed-Space" />
    <rdfs:subClassOf>
      <owl:Restriction> 
        <owl:onProperty rdf:resource="#is-part-of" />
        <owl:allValuesFrom rdf:resource="#Floor" />
      </owl:Restriction>
    </rdfs:subClassOf>
  </owl:Class>



  <!-- Types of room -->

  <owl:Class rdf:ID="Office">
    <rdfs:label>Office</rdfs:label>
    <rdfs:comment>This class is used to represent an Office, usually inhabited by a small number of people</rdfs:comment>
    <rdfs:subClassOf rdf:resource="#Room" />
  </owl:Class>

  <owl:Class rdf:ID="Laboratory">
    <rdfs:label>Laboratory</rdfs:label>
    <rdfs:comment>This class is used to represent a Laboratory, usually inhabited by a large number of people</rdfs:comment>
    <rdfs:subClassOf rdf:resource="#Room" />
  </owl:Class>

  <owl:Class rdf:ID="Meeting-Room">
    <rdfs:label>Meeting Room</rdfs:label>
    <rdfs:comment>This class is used to represent a room used for meetings</rdfs:comment>
    <rdfs:subClassOf rdf:resource="#Room" />
  </owl:Class>


  <!-- A Corridor -->

  <owl:Class rdf:ID="Corridor">
    <rdfs:label>Corridor</rdfs:label>
    <rdfs:comment>This class is used to represent a corridor, on a Floor of a Building</rdfs:comment>
    <rdfs:subClassOf rdf:resource="#Enclosed-Space" />
    <rdfs:subClassOf>
      <owl:Restriction>
        <owl:onProperty rdf:resource="#is-part-of" />
        <owl:allValuesFrom rdf:resource="#Floor" />
      </owl:Restriction>
    </rdfs:subClassOf>
  </owl:Class>
 

  <!-- Floor-Traversing-Spaces -->

  <owl:Class rdf:ID="Floor-Traversing-Space">
    <rdfs:label>Floor Traversing Space</rdfs:label>
    <rdfs:comment>This class is used to represent a space which traverses Floors</rdfs:comment>
    <rdfs:subClassOf rdf:resource="#Enclosed-Space" />
    <rdfs:subClassOf>
      <owl:Restriction>
        <owl:onProperty rdf:resource="#is-part-of" />
        <owl:allValuesFrom rdf:resource="#Building" />
      </owl:Restriction>
    </rdfs:subClassOf>
  </owl:Class>  

  <owl:Class rdf:ID="Stairs">
    <rdfs:label>Stairs</rdfs:label>
    <rdfs:comment>This class is used to represent Stairs, which traverse between Floors</rdfs:comment>
    <rdfs:subClassOf rdf:resource="#Floor-Traversing-Space" />
  </owl:Class>   

  <owl:Class rdf:ID="Lift">
    <rdfs:label>Lift</rdfs:label>
    <rdfs:comment>This class is used to represent a lift, which traverses between Floors</rdfs:comment>
    <rdfs:subClassOf rdf:resource="#Floor-Traversing-Space" />
  </owl:Class>



  <!-- A Partitioned-Space -->

  <owl:Class rdf:ID="Partitioned-Space">
    <rdfs:label>Partitioned Space</rdfs:label>
    <rdfs:comment>This class is used to represent a partitioned space in a Building. This is an Enclosed-Space, like a room, but which may permit communication between Partitioned-Spaces</rdfs:comment>
    <rdfs:subClassOf rdf:resource="#Enclosed-Space" />
    <rdfs:subClassOf>
      <owl:Restriction>
        <owl:onProperty rdf:resource="#is-part-of" />
        <owl:allValuesFrom rdf:resource="#Enclosed-Space" />
      </owl:Restriction>
    </rdfs:subClassOf>
  </owl:Class>



  <!--  Coordinate-Positions  -->

  <owl:Class rdf:ID="Coordinate-Position">
    <rdfs:label>Coordinate Position</rdfs:label>
    <rdfs:comment>This class is used as an abstract class, with the two sub-classes Relative-Coordinate-Position and GPS-Coordinate-Position</rdfs:comment>
  </owl:Class>



  <!--  Relative coordinate position -->

  <owl:Class rdf:ID="Relative-Coordinate-Position">
    <rdfs:label>Relative Coordinate Position</rdfs:label>
    <rdfs:comment>This position is described as an offset from the origin of another location</rdfs:comment>
    <rdfs:subClassOf rdf:resource="#Coordinate-Position"/>
  </owl:Class>

  <owl:DatatypeProperty rdf:ID="x-displacement">
    <rdfs:label>x displacement</rdfs:label>
    <rdfs:comment>The X displacement from the origin of another location</rdfs:comment>
    <rdfs:domain rdf:resource="#Relative-Coordinate-Position"/>
    <rdfs:range rdf:resource="&xsd;decimal"/>
  </owl:DatatypeProperty>

  <owl:DatatypeProperty rdf:ID="y-displacement">
    <rdfs:label>y displacement</rdfs:label>
    <rdfs:comment>The Y displacement from the origin of another location</rdfs:comment>
    <rdfs:domain rdf:resource="#Relative-Coordinate-Position"/>
    <rdfs:range rdf:resource="&xsd;decimal"/>
  </owl:DatatypeProperty>

  <owl:DatatypeProperty rdf:ID="z-displacement">
    <rdfs:label>z displacement</rdfs:label>
    <rdfs:comment>The Z displacement from the origin of another location</rdfs:comment>
    <rdfs:domain rdf:resource="#Relative-Coordinate-Position"/>
    <rdfs:range rdf:resource="&xsd;decimal"/>
  </owl:DatatypeProperty>

  <owl:ObjectProperty rdf:ID="relative-to-origin-of">
    <rdfs:label>relative to origin of</rdfs:label>
    <rdfs:comment>Location from which the relative position is derrived</rdfs:comment>
    <rdfs:domain rdf:resource="#Relative-Coordinate-Position"/>
    <rdfs:range rdf:resource="#Abstract-Space-With-Origin"/>
  </owl:ObjectProperty>



  <!--  GPS coordinate position -->

  <owl:Class rdf:ID="GPS-Coordinate-Position">
    <rdfs:label>GPS Coordinate Position</rdfs:label>
    <rdfs:comment>This position is a lat/long/alt GPS coordinate location</rdfs:comment>
    <owl:equivalentClass rdf:resource="&portal;Coordinate-Location"/>
    <rdfs:subClassOf rdf:resource="#Coordinate-Position"/>
  </owl:Class>

</rdf:RDF>
