<?xml version="1.0"?>

<!DOCTYPE owl [
  <!ENTITY xsd		"http://www.w3.org/2001/XMLSchema#">
  <!ENTITY rdf		"http://www.w3.org/1999/02/22-rdf-syntax-ns#">
  <!ENTITY rdfs		"http://www.w3.org/2000/01/rdf-schema#">
  <!ENTITY owl		"http://www.w3.org/2002/07/owl#">
  <!ENTITY base		"http://contextus.net/ontology/ontomedia/core/expression#">
  <!ENTITY dc           "http://purl.org/dc/elements/1.1/">
  <!ENTITY dct          "http://purl.org/dc/terms/">
  <!ENTITY locspec      "http://contextus.net/ontology/ontomedia/misc/locspec#">
  <!ENTITY omt	      	"http://contextus.net/ontology/ontomedia/ext/common/trait#">
  <!ENTITY dat	      	"http://contextus.net/ontology/ontomedia/misc/date#">
]>  



<rdf:RDF xmlns:rdf="&rdf;"
	 xmlns:rdfs="&rdfs;"
	 xmlns:owl="&owl;"
	 xmlns:xsd="&xsd;"
	 xmlns:locspec="&locspec;"
	 xmlns:dat="&dat;"
	 xml:base="&base;"
	 xml:omt="&omt;"
	 xmlns:dc="&dc;"
	 xmlns:dct="&dct;">

	 
  <owl:Ontology rdf:about="&base;">
    <rdfs:label>OntoMedia Core</rdfs:label>
    <dc:title xml:lang="en">OntoMedia Core</dc:title>
    <dc:description xml:lang="en">OntoMedia (Ontology for Media) has been designed to describe the interactions occurring in multimedia.</dc:description>
    <dc:creator>Michael O. Jewell (mailto:moj@ecs.soton.ac.uk)</dc:creator>
    <dc:creator>K Faith Lawrence (mailto:kf03r@ecs.soton.ac.uk)</dc:creator>
    <dc:creator>Mischa M Tuffield (mailto:mmt04r@ecs.soton.ac.uk)</dc:creator>
    <dct:created>2005-05-03</dct:created>
    <owl:versionInfo>0.32</owl:versionInfo>
  </owl:Ontology>

<!-- Core -->
  
  <owl:Class rdf:ID="Expression">
    <rdfs:label>Expression</rdfs:label>
    <rdfs:comment>This class represents a piece of information conveyed through a media</rdfs:comment>
   <!--  <rdfs:subClassOf rdf:resource="#Content" /> -->
  </owl:Class>
 
  <!-- Linking Properties -->

  <owl:ObjectProperty rdf:ID="is-linked-to">
    <rdfs:label>Is Linked To</rdfs:label>
    <rdfs:comment>This property indicates that there is some type of link between the named Expressions</rdfs:comment>
    <owl:inverseOf rdf:resource="#is-not-linked-to"/>
    <rdfs:domain rdf:resource="#Expression"/>
    <rdfs:range rdf:resource="#Expression"/>
  </owl:ObjectProperty>

  <owl:ObjectProperty rdf:ID="is-not-linked-to">
    <rdfs:label>Is Not Linked To</rdfs:label>
    <rdfs:comment>This property indicates that there is some no link between the named Expressions</rdfs:comment>
    <owl:inverseOf rdf:resource="#is-linked-to"/>
    <rdfs:domain rdf:resource="#Expression"/>
    <rdfs:range rdf:resource="#Expression"/>
  </owl:ObjectProperty>

  <owl:ObjectProperty rdf:ID="contains">
    <rdfs:label>Contains</rdfs:label>
    <rdfs:comment>This property indicates that one expression contains the other</rdfs:comment>
    <owl:inverseOf rdf:resource="#contained-by"/>
    <rdfs:subPropertyOf rdf:resource="#is-linked-to" />
    <rdfs:range rdf:resource="#Expression"/>
    <rdfs:domain rdf:resource="#Expression"/>
  </owl:ObjectProperty>

  <owl:ObjectProperty rdf:ID="contained-by">
    <rdfs:label>Contained By</rdfs:label>
    <rdfs:comment>This property indicates that one expression is contained by the other</rdfs:comment>
    <owl:inverseOf rdf:resource="#contains"/>
    <rdfs:subPropertyOf rdf:resource="#is-linked-to" />
    <rdfs:range rdf:resource="#Expression"/>
    <rdfs:domain rdf:resource="#Expression"/>
  </owl:ObjectProperty>
  
  <!-- Is the thing -->
  
  <owl:ObjectProperty rdf:ID="is">
    <rdfs:label>Is</rdfs:label>
    <rdfs:comment>This property indicates that the expression is exactly the same as another</rdfs:comment>
    <rdfs:subPropertyOf rdf:resource="#is-linked-to" />
    <owl:inverseOf rdf:resource="#is"/>
    <rdfs:domain rdf:resource="#Expression"/>
    <rdfs:range rdf:resource="#Expression"/>
  </owl:ObjectProperty>

  <owl:ObjectProperty rdf:ID="is-not">
    <rdfs:label>Is Not</rdfs:label>
    <rdfs:comment>This property indicates that the expression is entirely different to another</rdfs:comment>
    <rdfs:subPropertyOf rdf:resource="#is-not-linked-to" />
    <owl:inverseOf rdf:resource="#is-not"/>
    <rdfs:domain rdf:resource="#Expression"/>
    <rdfs:range rdf:resource="#Expression"/>
  </owl:ObjectProperty>

  <!-- Is similar/related to the thing -->

  <owl:ObjectProperty rdf:ID="has-variant">
    <rdfs:label>Has Variant</rdfs:label>
    <rdfs:comment>This property indicates that the expression is a variation of another</rdfs:comment>
    <rdfs:subPropertyOf rdf:resource="#is-linked-to" />
    <owl:inverseOf rdf:resource="has-variant"/>
    <rdfs:range rdf:resource="#Expression"/>
    <rdfs:domain rdf:resource="#Expression"/>
  </owl:ObjectProperty>

  <owl:ObjectProperty rdf:ID="has-shadow">
    <rdfs:label>Has Shadow</rdfs:label>
    <rdfs:comment>This property indicates that the expression is a variation on another, very similar but not exactly the same. For example the different interpretations of the same character</rdfs:comment>
    <rdfs:subPropertyOf rdf:resource="#has-variant" />
    <owl:inverseOf rdf:resource="#is-shadow-of"/>
    <rdfs:range rdf:resource="#Expression"/>
    <rdfs:domain rdf:resource="#Expression"/>
  </owl:ObjectProperty>

  <owl:ObjectProperty rdf:ID="is-shadow-of">
    <rdfs:label>Is Shadow Of</rdfs:label>
    <rdfs:comment>This property indicates that the expression is a variation on another, very similar but not exactly the same. For example the different interpretations of the same character</rdfs:comment>
    <rdfs:subPropertyOf rdf:resource="#has-variant" />
    <owl:inverseOf rdf:resource="#has-shadow"/>
    <rdfs:range rdf:resource="#Expression"/>
    <rdfs:domain rdf:resource="#Expression"/>
  </owl:ObjectProperty>
  
  <owl:ObjectProperty rdf:ID="has-spin-off">
    <rdfs:label>Has Spin Off</rdfs:label>
    <rdfs:comment>This property indicates that the expression has developed from another</rdfs:comment>
    <rdfs:subPropertyOf rdf:resource="#has-variant" />
    <owl:inverseOf rdf:resource="#is-spin-off-of"/>
    <rdfs:domain rdf:resource="#Item"/>
    <rdfs:range rdf:resource="#Item"/>
  </owl:ObjectProperty>

  <owl:ObjectProperty rdf:ID="is-spin-off-of">
    <rdfs:label>Is Spin Off Of</rdfs:label>
    <rdfs:comment>This property indicates that the expression has developed from another</rdfs:comment>
    <rdfs:subPropertyOf rdf:resource="#has-variant" />
    <owl:inverseOf rdf:resource="#has-spin-off"/>
   <rdfs:domain rdf:resource="#Item"/>
   <rdfs:range rdf:resource="#Item"/>
  </owl:ObjectProperty>
 
  <owl:ObjectProperty rdf:ID="inspired-by">
    <rdfs:label>Inspired By</rdfs:label>
    <rdfs:comment>This property indicates that the expression was inspired by another</rdfs:comment>
    <rdfs:subPropertyOf rdf:resource="#has-variant" />
    <owl:inverseOf rdf:resource="#inspired"/>
    <rdfs:domain rdf:resource="#Expression"/>
    <rdfs:range rdf:resource="#Expression"/>
  </owl:ObjectProperty>   

  <owl:ObjectProperty rdf:ID="inspired">
    <rdfs:label>Inspired</rdfs:label>
    <rdfs:comment>This property indicates that the expression inspired another</rdfs:comment>
    <rdfs:subPropertyOf rdf:resource="#has-variant" />
    <owl:inverseOf rdf:resource="#inspired-by"/>
    <rdfs:domain rdf:resource="#Expression"/>
    <rdfs:range rdf:resource="#Expression"/>
  </owl:ObjectProperty>

  <owl:ObjectProperty rdf:ID="is-potentially">
    <rdfs:label>Is Potentially</rdfs:label>
    <rdfs:subPropertyOf rdf:resource="#has-variant" />
    <rdfs:range rdf:resource="#Expression"/>
    <rdfs:domain rdf:resource="#Expression"/>
    <rdfs:comment>This property indicates that the expression is potentially another. For example, it may be a possible future version</rdfs:comment>
  </owl:ObjectProperty>
  
  <owl:ObjectProperty rdf:ID="refers-to">
    <rdfs:label>Refers To</rdfs:label>
    <rdfs:range rdf:resource="#Expression"/>
    <rdfs:domain rdf:resource="#Expression"/>
    <owl:inverseOf rdf:resource="#referenced-by"/>
    <rdfs:comment>This property indicates that the expression refers to another expression. This may be an event referring to a location, or a character refering to an event, etc.</rdfs:comment>
  </owl:ObjectProperty>
  
  <owl:ObjectProperty rdf:ID="referenced-by">
    <rdfs:label>Refers To</rdfs:label>
    <rdfs:range rdf:resource="#Expression"/>
    <rdfs:domain rdf:resource="#Expression"/>
    <owl:inverseOf rdf:resource="#refers-to"/>
    <rdfs:comment>This property indicates that the expression is refered to by another expression.</rdfs:comment>
  </owl:ObjectProperty>

  <!-- Entities -->
 
  <owl:Class rdf:ID="Entity">
    <rdfs:label>Entity</rdfs:label>
    <rdfs:comment>A thing</rdfs:comment>
    <rdfs:subClassOf rdf:resource="#Expression" />
    
  </owl:Class>

  <!-- Entity Subclasses -->

  <!-- Items -->

  <owl:Class rdf:ID="Item">
    <rdfs:comment>This class represents an entity which may participate in an event within the media. An Item may be abstract or physical</rdfs:comment>
    <rdfs:label>Item</rdfs:label>
    <rdfs:subClassOf rdf:resource="#Entity" />
  </owl:Class>
  
  
  <owl:Class rdf:ID="Physical-Item">
    <rdfs:comment>This class represents a physical entity which may participate in an event within the media</rdfs:comment>
    <rdfs:label>Physical Item</rdfs:label>
    <rdfs:subClassOf rdf:resource="#Item" />
    <rdfs:subClassOf rdf:resource="#Collection" />
  </owl:Class>
  
  <owl:Class rdf:ID="Abstract-Item">
    <rdfs:comment>This class represents an abstract entity which may participate in an event within the media</rdfs:comment>
    <rdfs:label>Abstract Item</rdfs:label>
    <rdfs:subClassOf rdf:resource="#Item" />
  </owl:Class>

  <!-- Abstract-Item Subclases -->
  
  <owl:Class rdf:ID="Context">
    <rdfs:comment>This class represents the context in which an event or entity exists</rdfs:comment>
    <rdfs:label>Context</rdfs:label>
    <rdfs:subClassOf rdf:resource="#Abstract-Item" />
  </owl:Class>  

  <owl:Class rdf:ID="Collection">
    <rdfs:comment>This class represents a collection of entities</rdfs:comment>
    <rdfs:label>Collection</rdfs:label>
    <rdfs:subClassOf rdf:resource="#Abstract-Item" />
  </owl:Class>  

 <!-- Context Properties -->
 
  <owl:ObjectProperty rdf:ID="allows-existence-of">
    <rdfs:comment>This class represents that the desired expression may exist within the context</rdfs:comment>
    <rdfs:label>Allows Existence Of</rdfs:label>  
    <rdfs:domain rdf:resource="&base;Context" />
    <owl:inverseOf rdf:resource="&base;exists-in"/>
    <rdfs:range rdf:resource="&base;Expression"/>
  </owl:ObjectProperty>

  <owl:ObjectProperty rdf:ID="exists-in">
    <rdfs:comment>This class represents that the expression exists within the related context</rdfs:comment>
    <rdfs:label>Exists In</rdfs:label> 
    <rdfs:domain rdf:resource="&base;Expression"/>
    <owl:inverseOf rdf:resource="&base;allows-existence-of"/>
    <rdfs:range rdf:resource="&base;Context"/>
  </owl:ObjectProperty> 
  
  <!-- Collection Properties -->
  
  <owl:ObjectProperty rdf:ID="has-number-of-parts">
      <rdfs:label>Has Number Of Parts</rdfs:label>
      <rdfs:comment>This property specifies the number of parts contained by the collection</rdfs:comment>
      <rdfs:domain rdf:resource="&base;Collection"/>
      <rdfs:range rdf:resource="&rdfs;Literal"/>
  </owl:ObjectProperty> 
  
  <owl:ObjectProperty rdf:ID="has-max-number-of-parts">
      <rdfs:label>Has Maximum Number Of Parts</rdfs:label>
      <rdfs:comment>This property specifies the maximum number of parts that can be contained by the collection</rdfs:comment>
      <rdfs:domain rdf:resource="&base;Collection"/>
      <rdfs:range rdf:resource="&rdfs;Literal"/>
  </owl:ObjectProperty> 
  
  <owl:ObjectProperty rdf:ID="has-min-number-of-parts">
        <rdfs:label>Has Minimum Number Of Parts</rdfs:label>
        <rdfs:comment>This property specifies the minimum number of parts that can be contained by the collection</rdfs:comment>
        <rdfs:domain rdf:resource="&base;Collection"/>
        <rdfs:range rdf:resource="&rdfs;Literal"/>
  </owl:ObjectProperty> 
  

  <!-- Temporal -->
  
  <owl:Class rdf:ID="Timeline">
    <rdfs:comment>This class contains a sequence of occurring events</rdfs:comment>
    <rdfs:label>Timeline</rdfs:label>
    <rdfs:subClassOf rdf:resource="#Entity" />
  </owl:Class>

  <owl:Class rdf:ID="Occurrence">
    <rdfs:comment>This class represents a single occurrence of an event, placing it at a position in a timeline</rdfs:comment>
    <rdfs:label>Occurrence</rdfs:label>
    <rdfs:subClassOf rdf:resource="#Entity" />
  </owl:Class>
  
  <!-- Temporal Properties -->
  
  <owl:ObjectProperty rdf:ID="timeline-ref">
    <rdfs:label>Timeline Reference</rdfs:label>
    <rdfs:comment>Reference to the Timeline that the Occurrence exists on</rdfs:comment>  
    <rdfs:range rdf:resource="#Timeline"/>
    <rdfs:domain rdf:resource="#Occurrence"/>
  </owl:ObjectProperty>  
  
  <owl:ObjectProperty rdf:ID="occurrence-of">
    <rdfs:label>Occurrence Of</rdfs:label>
    <rdfs:comment>This property defines any the event that the occurrence relates to</rdfs:comment>
    <owl:inverseOf rdf:resource="#has-occurrence"/>
    <rdfs:domain rdf:resource="#Occurrence"/>
    <rdfs:range rdf:resource="#Event"/>
  </owl:ObjectProperty>
  
  <owl:ObjectProperty rdf:ID="precedes">
    <rdfs:label>Precedes</rdfs:label>
    <rdfs:comment>This property defines the occurrence which immediately follows this occurrence</rdfs:comment>
    <rdfs:range rdf:resource="#Occurrence"/>
    <rdfs:domain rdf:resource="#Occurrence"/>
    <owl:inverseOf rdf:resource="#follows"/>
  </owl:ObjectProperty>
  
  <owl:ObjectProperty rdf:ID="follows">
    <rdfs:label>Follows</rdfs:label>
    <rdfs:comment>Follows specifies the occurrence that happens after the referencing occurrence</rdfs:comment>
    <rdfs:range rdf:resource="#Occurrence"/>
    <rdfs:domain rdf:resource="#Occurrence"/>
    <owl:inverseOf rdf:resource="#precedes"/>
  </owl:ObjectProperty>
  
  <!-- Time References -->

  <owl:ObjectProperty rdf:ID="TAQ">
    <rdfs:label>Period Terminal Limit</rdfs:label>
    <rdfs:comment>Terminus Ante Quem (Limit Before Which): The latest date that the period the event covers could have happened</rdfs:comment>
    <rdfs:domain rdf:resource="#Occurrence"/>
    <rdfs:range rdf:resource="&dat;Date"/>
  </owl:ObjectProperty>

  <owl:ObjectProperty rdf:ID="TPQ">
    <rdfs:label>Temporal Start</rdfs:label>
    <rdfs:comment>The time/date/temporal reference for the start of the event</rdfs:comment>
    <rdfs:range rdf:resource="&dat;Date"/>
    <rdfs:domain rdf:resource="#Occurrence"/>
  </owl:ObjectProperty>

  <owl:ObjectProperty rdf:ID="StartTime">
    <rdfs:label>Temporal End</rdfs:label>
    <rdfs:comment>The time/date/temporal reference for the start of the event</rdfs:comment>
    <rdfs:domain rdf:resource="#Occurrence"/>
    <rdfs:range rdf:resource="&dat;Date"/>
  </owl:ObjectProperty>

  <owl:ObjectProperty rdf:ID="EndTime">
    <rdfs:label>Period Initial Limit</rdfs:label>
    <rdfs:comment>The time/date/temporal reference for the end of the event</rdfs:comment>
    <rdfs:range rdf:resource="&dat;Date"/>
    <rdfs:domain rdf:resource="#Occurrence"/>
  </owl:ObjectProperty>

  <owl:ObjectProperty rdf:ID="DiscreteTime">
    <rdfs:label>Time/Date</rdfs:label>
    <rdfs:comment>The time/date/temporal reference for the the event</rdfs:comment>
    <rdfs:domain rdf:resource="#Occurrence"/>
    <rdfs:range rdf:resource="&dat;Date"/>
  </owl:ObjectProperty>
  
  <!-- Links to Media -->
  
  <owl:FunctionalProperty rdf:ID="occurs">
    <rdfs:label>Occurs</rdfs:label>
    <rdfs:comment>This property specifies the region of media in when an event occurrence happens</rdfs:comment>
    <rdfs:range rdf:resource="&locspec;LocSpec"/>
    <rdfs:domain rdf:resource="#Occurrence"/>
  </owl:FunctionalProperty>
    
  <owl:FunctionalProperty rdf:ID="start-point">
    <rdfs:label>Start point in Media</rdfs:label>
    <rdfs:comment>This property specifies the point in the media at which the event occurrence starts happening</rdfs:comment>
    <rdfs:domain rdf:resource="#Occurrence"/>
    <rdfs:range rdf:resource="&locspec;LocSpec"/>
  </owl:FunctionalProperty>
  
  <owl:FunctionalProperty rdf:ID="has-duration">
    <rdfs:label>Duration of Occurrence</rdfs:label>
    <rdfs:comment>This property specifies the duration of the occurrence</rdfs:comment>
    <rdfs:domain rdf:resource="#Occurrence"/>
    <rdfs:range>
      <owl:Class>
        <owl:unionOf rdf:parseType="Collection">
          <owl:Class rdf:about="&locspec;LocSpec"/>
          <owl:Class rdf:about="&omt;Dimension"/>
        </owl:unionOf>
      </owl:Class>
    </rdfs:range>
  </owl:FunctionalProperty>
  
  <owl:ObjectProperty rdf:ID="end-point">
    <rdfs:label>End Point in Media</rdfs:label>
    <rdfs:comment>This property specifies the point in the media at which the event occurrence stops happening</rdfs:comment>
    <rdfs:range rdf:resource="&locspec;LocSpec"/>
    <rdfs:domain rdf:resource="#Occurrence"/>
  </owl:ObjectProperty>

  <owl:ObjectProperty rdf:ID="MediaTPQ">
    <rdfs:label>Media Start Period Limit</rdfs:label>
    <rdfs:comment>This property specifies the earliest point in the media at which the event occurrence could have happened</rdfs:comment>
    <rdfs:range rdf:resource="&locspec;LocSpec"/>
    <rdfs:comment>Terminus Post Quem (Limit After Which): The earliest point that the period the event covers could be said to be happening</rdfs:comment>
    <rdfs:domain rdf:resource="#Occurrence"/>
  </owl:ObjectProperty>
  
  <owl:ObjectProperty rdf:ID="MediaTAQ">
    <rdfs:label>Media End Period Limit</rdfs:label>
    <rdfs:comment>Terminus Ante Quem (Limit Before Which): The latest point that the period the event covers could have happened</rdfs:comment>
    <rdfs:domain rdf:resource="#Occurrence"/>
    <rdfs:range rdf:resource="&locspec;LocSpec"/>
  </owl:ObjectProperty>
  
  <!-- Events -->

  <owl:Class rdf:ID="Event">
    <rdfs:label>Event</rdfs:label>
    <rdfs:comment>This property defines an event</rdfs:comment>
    <rdfs:subClassOf rdf:resource="#Expression" />
  </owl:Class>

  <!-- Event Properties -->
  
  <owl:ObjectProperty rdf:ID="final-event">
    <rdfs:domain rdf:resource="#Event"/>
    <rdfs:range rdf:resource="#Event"/>
  </owl:ObjectProperty>
  
  <owl:ObjectProperty rdf:ID="initial-event">
    <rdfs:comment
    >the first event which begins this sequence</rdfs:comment>
    <rdfs:domain rdf:resource="#Event"/>
    <rdfs:range rdf:resource="#Event"/>
  </owl:ObjectProperty>  
  
  <owl:ObjectProperty rdf:ID="has-subject-entity">
    <rdfs:label>Has Subject Entity</rdfs:label>
    <rdfs:comment>This property specifies the entity which carries out the aim of the event</rdfs:comment>
    <rdfs:domain rdf:resource="#Event"/>
    <rdfs:range rdf:resource="#Entity"/>
  </owl:ObjectProperty>
  
  <owl:ObjectProperty rdf:ID="has-object-entity">
    <rdfs:label>Has Object Entity</rdfs:label>
    <rdfs:comment>This property specifies the entity which is the target of the event</rdfs:comment>
    <rdfs:range rdf:resource="#Entity"/>
    <rdfs:domain rdf:resource="#Event"/>
  </owl:ObjectProperty>

  
  <owl:ObjectProperty rdf:ID="has-occurrence">
    <rdfs:label>Has occurrence</rdfs:label>
    <rdfs:comment>This property defines any occurrences of this event</rdfs:comment>
    <rdfs:range rdf:resource="#Occurrence"/>
    <rdfs:domain rdf:resource="#Event" />
    <owl:inverseOf rdf:resource="#occurrence-of"/>
  </owl:ObjectProperty> 
  
  <owl:FunctionalProperty rdf:ID="summary">
    <rdfs:label>Summary</rdfs:label>
    <rdfs:domain rdf:resource="#Event"/>
    <rdfs:range rdf:resource="&rdfs;Literal"/>
    <rdfs:comment>This property is a plain-text summery of what occurs in the event</rdfs:comment>
  </owl:FunctionalProperty>
  
  <owl:ObjectProperty rdf:ID="precondition">
    <rdfs:label>Precondition</rdfs:label>
    <rdfs:comment>This property is a state that must exist before the event can occur</rdfs:comment>
    <rdfs:range>
      <owl:Class>
        <owl:unionOf rdf:parseType="Collection">
          <owl:Class rdf:about="#Entity"/>
          <owl:Class rdf:about="#Event"/>
        </owl:unionOf>
      </owl:Class>
    </rdfs:range>
    <rdfs:domain rdf:resource="#Event"/>
  </owl:ObjectProperty>
  
  <owl:ObjectProperty rdf:ID="postcondition">
    <rdfs:label>Postcondition</rdfs:label>
    <rdfs:range>
      <owl:Class>
        <owl:unionOf rdf:parseType="Collection">
          <owl:Class rdf:about="#Entity"/>
          <owl:Class rdf:about="#Event"/>
        </owl:unionOf>
      </owl:Class>
    </rdfs:range>
    <rdfs:comment>This property contains the state which should occur as a consequence of this event</rdfs:comment>
    <rdfs:domain rdf:resource="#Event"/>
  </owl:ObjectProperty>

  <owl:ObjectProperty rdf:ID="involves">
    <rdfs:label>Involves</rdfs:label>
    <rdfs:comment>This property specifies the entities involved in this event. Note that this includes the subject and object.</rdfs:comment>
    <rdfs:range rdf:resource="#Entity"/>
    <rdfs:domain rdf:resource="#Event"/>
    <owl:inverseOf rdf:resource="#involved-in" />
  </owl:ObjectProperty>

  <owl:ObjectProperty rdf:ID="involved-in">
    <rdfs:label>Involves</rdfs:label>
    <rdfs:comment>This property specifies the events involved in by this entity. Note that this includes the subject and object.</rdfs:comment>
    <rdfs:range rdf:resource="#Event"/>
    <rdfs:domain rdf:resource="#Entity"/>
    <owl:inverseOf rdf:resource="#involves" />
  </owl:ObjectProperty>

  <owl:ObjectProperty rdf:ID="causes">
    <rdfs:label>Causes</rdfs:label>
    <rdfs:comment>This property indicates the instigating factor of an event, whether it be an item, event, or collection.</rdfs:comment>
    <rdfs:range>
      <owl:Class>
        <owl:unionOf rdf:parseType="Collection">
          <owl:Class rdf:about="#Event"/>
          <owl:Class rdf:about="#Entity"/>
        </owl:unionOf>
      </owl:Class>
    </rdfs:range>
    <rdfs:domain>
      <owl:Class>
        <owl:unionOf rdf:parseType="Collection">
          <owl:Class rdf:about="#Event"/>
          <owl:Class rdf:about="#Entity"/>
        </owl:unionOf>
      </owl:Class>
    </rdfs:domain>
    <owl:inverseOf rdf:resource="#caused-by"/>
  </owl:ObjectProperty>

  <owl:ObjectProperty rdf:ID="caused-by">
    <rdfs:label>Caused By</rdfs:label>
    <rdfs:comment>This property indicates the instigating factor of an event, whether it be an item, event, or collection.</rdfs:comment>
    <rdfs:range>
      <owl:Class>
        <owl:unionOf rdf:parseType="Collection">
          <owl:Class rdf:about="#Event"/>
          <owl:Class rdf:about="#Entity"/>
        </owl:unionOf>
      </owl:Class>
    </rdfs:range>
    <rdfs:domain>
      <owl:Class>
        <owl:unionOf rdf:parseType="Collection">
          <owl:Class rdf:about="#Event"/>
          <owl:Class rdf:about="#Entity"/>
        </owl:unionOf>
      </owl:Class>
    </rdfs:domain>
    <owl:inverseOf rdf:resource="#causes"/>
  </owl:ObjectProperty>


  <!-- Event Subclasses -->

  
  <owl:Class rdf:ID="Gain">
    <rdfs:label>Gain</rdfs:label>
    <rdfs:subClassOf rdf:resource="#Event" />
    <rdfs:comment>This event class results in an overall increase of the entities related to the primary subject or subjects of the event</rdfs:comment>
  </owl:Class>
  
  <owl:Class rdf:ID="Introduction">
    <rdfs:label>Introduction</rdfs:label>
    <rdfs:comment>This event class denotes the introduction of an entity to the media</rdfs:comment>
    <rdfs:subClassOf rdf:resource="#Event" />
  </owl:Class>
  
  <owl:Class rdf:ID="Loss">
    <rdfs:label>Loss</rdfs:label>
    <rdfs:comment>This event class results in an overall reduction of the entities related to the primary subject or subjects of the event</rdfs:comment>
    <rdfs:subClassOf rdf:resource="#Event" />
  </owl:Class>
  
  <owl:Class rdf:ID="Transformation">
    <rdfs:comment>This event class results in no gain or loss of attributes or entities, merely alteration</rdfs:comment>
    <rdfs:label>Transformation</rdfs:label>
    <rdfs:subClassOf rdf:resource="#Event" />
  </owl:Class>

  <owl:Class rdf:ID="Action">
    <rdfs:comment>This event class describes an action sequence (ie no plot)</rdfs:comment>
    <rdfs:label>Action</rdfs:label>
    <rdfs:subClassOf rdf:resource="#Event" />
  </owl:Class>

  <owl:Class rdf:ID="Social">
    <rdfs:comment>This event class describes a sequence focusing on social, interpersonal and personal emotional elements</rdfs:comment>
    <rdfs:label>Social</rdfs:label>
    <rdfs:subClassOf rdf:resource="#Event" />
  </owl:Class>
  
  <!-- Transformation Properties -->
  
  <owl:ObjectProperty rdf:ID="from">
    <rdfs:label>From</rdfs:label>
    <rdfs:comment>This property specifies the entity which is being transformed</rdfs:comment>
    <rdfs:range rdf:resource="#Entity" />
    <rdfs:domain rdf:resource="#Transformation" />
  </owl:ObjectProperty>
  
  <owl:ObjectProperty rdf:ID="to">
    <rdfs:label>To</rdfs:label>
    <rdfs:comment>This property specifies the resultant entity</rdfs:comment>
    <rdfs:range rdf:resource="#Entity" />
    <rdfs:domain rdf:resource="#Transformation" />
  </owl:ObjectProperty>
  
  
  <!-- Unsorted -->
<!--
  
  <owl:ObjectProperty rdf:ID="expresses">
    <rdfs:domain rdf:resource="#Expressible"/>
    <rdfs:range rdf:resource="#Expression"/>
  </owl:ObjectProperty>
-->  

  <!-- ????

  <owl:DatatypeProperty rdf:ID="type">
    <rdfs:range rdf:resource="&rdfs;Literal"/>
    <rdfs:domain rdf:resource="#Item"/>
  </owl:DatatypeProperty>
-->
 
</rdf:RDF>
