<?xml version="1.0"?>
<!DOCTYPE owl [
<!ENTITY base 	"http://www.r4isstatic.com/linkeddata/ontologies/ontomedia/misc/colour#">
<!ENTITY omt "http://www.r4isstatic.com/linkeddata/ontologies/ontomedia/ext/common/trait#">
<!ENTITY rdf 	"http://www.w3.org/1999/02/22-rdf-syntax-ns#">
<!ENTITY owl 	"http://www.w3.org/2002/07/owl#">
<!ENTITY rdfs 	"http://www.w3.org/2000/01/rdf-schema#">
<!ENTITY dc	"http://purl.org/dc/elements/1.1/">
<!ENTITY dct	"http://purl.org/dc/terms/">
<!ENTITY xsd	"http://www.w3.org/2001/XMLSchema#">
]>


<rdf:RDF
 xmlns:rdf="&rdf;"
 xmlns:owl="&owl;"
 xmlns:rdfs="&rdfs;"
 xml:base="&base;"
 xmlns:dc="&dc;"
 xmlns:dct="&dct;"
 xmlns:xsd="&xsd;"
 xmlns:omt="&omt;"
>

<owl:Ontology rdf:about="&base;">
 <rdfs:label>OntoMedia Colour Ontology</rdfs:label>

<dc:description xml:lang="en">This ontology provides a portable representation of colour.</dc:description>
  <dc:creator>Michael O. Jewell (mailto:moj@ecs.soton.ac.uk)</dc:creator>
  <dc:creator>K Faith Lawrence (mailto:kf03r@ecs.soton.ac.uk)</dc:creator>
  <dc:creator>Mischa M Tuffield (mailto:mmt04r@ecs.soton.ac.uk)</dc:creator>
  <dct:created>2005-05-27</dct:created>
  <owl:versionInfo>0.1</owl:versionInfo>
</owl:Ontology>

<!-- COLOUR DEFINED IN TRAITS

<owl:Class rdf:ID="Colour">
  <rdfs:label>Colour</rdfs:label>
  <rdfs:comment>A generic colour. This may have a number of shades.</rdfs:comment>
</owl:Class>

--> 

<owl:ObjectProperty rdf:ID="has-shade">
  <rdfs:label>Has Shade</rdfs:label>
  <rdfs:comment>This property specifies the shades which come under the label of this colour</rdfs:comment>
  <rdfs:domain rdf:resource="&omt;Colour" />
  <rdfs:range rdf:resource="&base;Shade" />
</owl:ObjectProperty>

<owl:Class rdf:ID="Shade">
  <rdfs:label>Shade</rdfs:label>
  <rdfs:subClassOf rdf:resource="&omt;Colour" />
  <rdfs:comment>A specific colour. This has hue, saturation and brightness.</rdfs:comment>
</owl:Class>

<owl:DatatypeProperty rdf:ID="has-hue">
  <rdfs:label>Has Hue</rdfs:label>
  <rdfs:comment>This property specifies the hue of a shade (from 0.0 to 360.0)</rdfs:comment>
  <rdfs:domain rdf:resource="&base;Shade" />
  <rdfs:range rdf:resource="&xsd;decimal" />
</owl:DatatypeProperty>

<owl:DatatypeProperty rdf:ID="has-saturation">
  <rdfs:label>Has Saturation</rdfs:label>
  <rdfs:comment>This property specifies the saturation of a shade (from 0.0 to 100.0)</rdfs:comment>
  <rdfs:domain rdf:resource="&base;Shade" />
  <rdfs:range rdf:resource="&xsd;decimal" />
</owl:DatatypeProperty>

<owl:DatatypeProperty rdf:ID="has-brightness">
  <rdfs:label>Has Brightness</rdfs:label>
  <rdfs:comment>This property specifies the brightness of a shade (from 0.0 to 100.0)</rdfs:comment>
  <rdfs:domain rdf:resource="&base;Shade" />
  <rdfs:range rdf:resource="&xsd;decimal" />
</owl:DatatypeProperty>


</rdf:RDF>  
