<?xml version="1.0"?>
<!DOCTYPE owl [
<!ENTITY ome "http://contextus.net/ontology/ontomedia/core/expression#">
<!ENTITY omt "http://contextus.net/ontology/ontomedia/ext/common/trait#">
<!ENTITY loc "http://contextus.net/ontology/ontomedia/core/space#">
<!ENTITY omea "http://contextus.net/ontology/ontomedia/ext/events/action#">
<!ENTITY omb "http://contextus.net/ontology/ontomedia/ext/common/being#">
<!ENTITY dc "http://purl.org/dc/elements/1.1/">
<!ENTITY dct "http://purl.org/dc/terms/">
<!ENTITY xsd "http://www.w3.org/2001/XMLSchema#">
<!ENTITY rdf "http://www.w3.org/1999/02/22-rdf-syntax-ns#">
<!ENTITY owl "http://www.w3.org/2002/07/owl#">
<!ENTITY rdfs "http://www.w3.org/2000/01/rdf-schema#">
<!ENTITY base "http://contextus.net/ontology/ontomedia/ext/common/profession#">
]>


<rdf:RDF
 xmlns:ome="&ome;"
 xmlns:omea="&omea;"
 xmlns:omt="&omt;"
 xmlns:omb="&omb;"
 xmlns:loc="&loc;"
 xmlns:dc="&dc;"
 xmlns:dct="&dct;"
 xmlns:xsd="&xsd;"
 xmlns:rdf="&rdf;"
 xmlns:owl="&owl;"
 xmlns:rdfs="&rdfs;"
 xml:base="&base;"
>
	 	 

<owl:Ontology rdf:about="&base;">
 <rdfs:label>Profession Extension</rdfs:label>
 <dc:title xml:lang="en">OntoMedia Profession Ontology</dc:title>
 <dc:description xml:lang="en">OntoMedia (Ontology for Media) Profession Extension has been designed to describe general profession categories.</dc:description>
 <dc:creator>K Faith Lawrence (mailto:kf03r@ecs.soton.ac.uk)</dc:creator>
 <dct:created>2006-04-05</dct:created>
 <owl:versionInfo>0.1</owl:versionInfo>
</owl:Ontology>

<!-- Events -->

<owl:Class rdf:ID="GainJob">
  <rdfs:subClassOf rdf:resource="&ome;Gain" />
  <rdfs:comment>This class represents a being gaining a job or prossesion</rdfs:comment>
  <rdfs:label>Gain Job/Employment</rdfs:label>
</owl:Class>

<owl:Class rdf:ID="LoseJob">
  <rdfs:subClassOf rdf:resource="&ome;Loss" />
  <rdfs:comment>This class represents a being losing a job or profession</rdfs:comment>
  <rdfs:label>Lose Job/Employment</rdfs:label>
</owl:Class>

<!-- Main Classes -->

<owl:Class rdf:ID="Clerical">
  <rdfs:subClassOf rdf:resource="&omb;Profession" />
  <rdfs:comment>This class represents clerical professions</rdfs:comment>
  <rdfs:label>Clerical</rdfs:label>
</owl:Class>

<owl:Class rdf:ID="Criminal">
  <rdfs:subClassOf rdf:resource="&omb;Profession" />
  <rdfs:comment>This class represents professions based on illegal activities</rdfs:comment>
  <rdfs:label>Criminal</rdfs:label>
</owl:Class>

<owl:Class rdf:ID="Domestic">
  <rdfs:subClassOf rdf:resource="&omb;Profession" />
  <rdfs:comment>This class represents domestic professions</rdfs:comment>
  <rdfs:label>Domestic</rdfs:label>
</owl:Class>

<owl:Class rdf:ID="Education">
  <rdfs:subClassOf rdf:resource="&omb;Profession" />
  <rdfs:comment>This class represents professions based on educational activities</rdfs:comment>
  <rdfs:label>Education</rdfs:label>
</owl:Class>

<owl:Class rdf:ID="Enforcement">
  <rdfs:subClassOf rdf:resource="&omb;Profession" />
  <rdfs:comment>This class represents enforcement professions</rdfs:comment>
  <rdfs:label>Enforcement</rdfs:label>
</owl:Class>

<owl:Class rdf:ID="Entertainment">
  <rdfs:subClassOf rdf:resource="&omb;Profession" />
  <rdfs:comment>This class represents professions based on entertaining activities</rdfs:comment>
  <rdfs:label>Entertainment</rdfs:label>
</owl:Class>

<owl:Class rdf:ID="Governance">
  <rdfs:subClassOf rdf:resource="&omb;Profession" />
  <rdfs:comment>This class represents professions involved in government</rdfs:comment>
  <rdfs:label>Governance</rdfs:label>
</owl:Class>

<owl:Class rdf:ID="Healthcare">
  <rdfs:subClassOf rdf:resource="&omb;Profession" />
  <rdfs:comment>This class represents professions based on healthcare activities</rdfs:comment>
  <rdfs:label>Healthcare</rdfs:label>
</owl:Class>

<owl:Class rdf:ID="Information-Services">
  <rdfs:subClassOf rdf:resource="&omb;Profession" />
  <rdfs:comment>This class represents professions based on information related activities</rdfs:comment>
  <rdfs:label>Information Services</rdfs:label>
</owl:Class>

<owl:Class rdf:ID="Manual">
  <rdfs:subClassOf rdf:resource="&omb;Profession" />
  <rdfs:comment>This class represents manual professions</rdfs:comment>
  <rdfs:label>Manual</rdfs:label>
</owl:Class>

<owl:Class rdf:ID="Religious">
  <rdfs:subClassOf rdf:resource="&omb;Profession" />
  <rdfs:comment>This class represents professions based on religious activities</rdfs:comment>
  <rdfs:label>Religious</rdfs:label>
</owl:Class>

<owl:Class rdf:ID="Rural">
  <rdfs:subClassOf rdf:resource="&omb;Profession" />
  <rdfs:comment>This class represents rural professions</rdfs:comment>
  <rdfs:label>Rural</rdfs:label>
</owl:Class>

<owl:Class rdf:ID="Trade">
  <rdfs:subClassOf rdf:resource="&omb;Profession" />
  <rdfs:comment>This class represents professions based on trading activities</rdfs:comment>
  <rdfs:label>Trade</rdfs:label>
</owl:Class>

<owl:Class rdf:ID="Unemployed">
  <rdfs:subClassOf rdf:resource="&omb;Profession" />
  <rdfs:comment>This class represents a lack of employment</rdfs:comment>
  <rdfs:label>Unemployed</rdfs:label>
</owl:Class>

<owl:Class rdf:ID="Volunteer">
  <rdfs:subClassOf rdf:resource="&omb;Profession" />
  <rdfs:comment>This class represents professions based on volunteer activities</rdfs:comment>
  <rdfs:label>Volunteer</rdfs:label>
</owl:Class>

<!-- Clerical -->

<owl:Class rdf:ID="Management">
  <rdfs:subClassOf rdf:resource="&base;Clerical" />
  <rdfs:comment>This class represents professions based on management activities</rdfs:comment>
  <rdfs:label>Manager</rdfs:label>
</owl:Class>

<!-- Education -->

<owl:Class rdf:ID="Student">
  <rdfs:subClassOf rdf:resource="&base;Education" />
  <rdfs:comment>This class represents professions based on learning activities</rdfs:comment>
  <rdfs:label>Student</rdfs:label>
</owl:Class>

<owl:Class rdf:ID="Teacher">
  <rdfs:subClassOf rdf:resource="&base;Education" />
  <rdfs:comment>This class represents professions based on teaching activities</rdfs:comment>
  <rdfs:label>Teacher</rdfs:label>
</owl:Class>

<!-- Enforcement -->

<owl:Class rdf:ID="Law-Enforcement">
  <rdfs:subClassOf rdf:resource="&base;Enforcement" />
  <rdfs:comment>This class represents professions based on enforcing the legal code of the region</rdfs:comment>
  <rdfs:label>Law Enforcement</rdfs:label>
</owl:Class>

<owl:Class rdf:ID="RegionalCops">
  <rdfs:subClassOf rdf:resource="&base;Law-Enforcement" />
  <rdfs:comment>This class represents professions based on enforcing the legal code of a country at a regional level</rdfs:comment>
  <rdfs:label>Regional Law Enforcement</rdfs:label>
</owl:Class>

<owl:Class rdf:ID="NationalCops">
  <rdfs:subClassOf rdf:resource="&base;Law-Enforcement" />
  <rdfs:comment>This class represents professions based on enforcing the legal code of a country at a national level</rdfs:comment>
  <rdfs:label>National Law Enforcement</rdfs:label>
</owl:Class>

<owl:Class rdf:ID="InternationalCops">
  <rdfs:subClassOf rdf:resource="&base;Law-Enforcement" />
  <rdfs:comment>This class represents professions based on enforcing international legal codes or legal codes at an international level</rdfs:comment>
  <rdfs:label>International Law Enforcement</rdfs:label>
</owl:Class>

<owl:Class rdf:ID="Military">
  <rdfs:subClassOf rdf:resource="&base;Enforcement" />
  <rdfs:comment>This class represents professions based on military activities</rdfs:comment>
  <rdfs:label>Military</rdfs:label>
</owl:Class>

<owl:Class rdf:ID="Regular-Military">
  <rdfs:subClassOf rdf:resource="&base;Military" />
  <rdfs:comment>This class represents professions based within the regular military</rdfs:comment>
  <rdfs:label>Regular Military</rdfs:label>
</owl:Class>

<owl:Class rdf:ID="Paramilitary">
  <rdfs:subClassOf rdf:resource="&base;Military" />
  <rdfs:comment>This class represents professions based on paramilitary activities</rdfs:comment>
  <rdfs:label>Paramilitary</rdfs:label>
</owl:Class>

<owl:Class rdf:ID="Special-Services">
  <rdfs:subClassOf rdf:resource="&base;Military" />
  <rdfs:comment>This class represents professions based on more irregular or unusual military activities</rdfs:comment>
  <rdfs:label>Special Services</rdfs:label>
</owl:Class>

<!-- Entertainment -->

<owl:Class rdf:ID="Acting">
  <rdfs:subClassOf rdf:resource="&base;Entertainment" />
  <rdfs:comment>This class represents professions based on acting</rdfs:comment>
  <rdfs:label>Acting</rdfs:label>
</owl:Class>

<owl:Class rdf:ID="VoiceActing">
  <rdfs:subClassOf rdf:resource="&base;Entertainment" />
  <rdfs:comment>This class represents professions based on voice acting</rdfs:comment>
  <rdfs:label>Voice Acting</rdfs:label>
</owl:Class>

<owl:Class rdf:ID="Artist">
  <rdfs:subClassOf rdf:resource="&base;Entertainment" />
  <rdfs:comment>This class represents professions relating to the creation of works of art</rdfs:comment>
  <rdfs:label>Artist</rdfs:label>
</owl:Class>

<owl:Class rdf:ID="Backstage-Crew">
  <rdfs:subClassOf rdf:resource="&base;Entertainment" />
  <rdfs:comment>This class represents professions based on the backstage/behind the scenes professions</rdfs:comment>
  <rdfs:label>Backstage Crew</rdfs:label>
</owl:Class>

<owl:Class rdf:ID="Dancer">
  <rdfs:subClassOf rdf:resource="&base;Entertainment" />
  <rdfs:comment>This class represents professions based on dancing</rdfs:comment>
  <rdfs:label>Dancer</rdfs:label>
</owl:Class>

<owl:Class rdf:ID="Musician">
  <rdfs:subClassOf rdf:resource="&base;Entertainment" />
  <rdfs:comment>This class represents professions based on performing music with a instrament</rdfs:comment>
  <rdfs:label>Musician</rdfs:label>
</owl:Class>

<owl:Class rdf:ID="Composer">
  <rdfs:subClassOf rdf:resource="&base;Musician" />
  <rdfs:comment>This class represents professions based on the composition of music</rdfs:comment>
  <rdfs:label>Composer</rdfs:label>
</owl:Class>

<owl:Class rdf:ID="Singer">
  <rdfs:subClassOf rdf:resource="&base;Entertainment" />
  <rdfs:comment>This class represents professions based on performing music with the voice</rdfs:comment>
  <rdfs:label>Singer</rdfs:label>
</owl:Class>

<owl:Class rdf:ID="Writer">
  <rdfs:subClassOf rdf:resource="&base;Entertainment" />
  <rdfs:comment>This class represents professions based on writing text</rdfs:comment>
  <rdfs:label>Writer</rdfs:label>
</owl:Class>

<owl:Class rdf:ID="Poet">
  <rdfs:subClassOf rdf:resource="&base;Entertainment" />
  <rdfs:comment>This class represents professions based on writing poetry</rdfs:comment>
  <rdfs:label>Poet</rdfs:label>
</owl:Class>

<!-- Governance -->

<owl:Class rdf:ID="Legislature">
  <rdfs:subClassOf rdf:resource="&base;Governance" />
  <rdfs:comment>This class represents professions based on legislating activities</rdfs:comment>
  <rdfs:label>Legislature</rdfs:label>
</owl:Class>

<owl:Class rdf:ID="Nobility">
  <rdfs:subClassOf rdf:resource="&base;Governance" />
  <rdfs:comment>This class represents the profession involving being part of the noble class</rdfs:comment>
  <rdfs:label>Nobility</rdfs:label>
</owl:Class>

<owl:Class rdf:ID="Ruler">
  <rdfs:subClassOf rdf:resource="&base;Governance" />
  <rdfs:comment>This class represents professions based on ruling</rdfs:comment>
  <rdfs:label>Ruler</rdfs:label>
</owl:Class>

<!-- Healthcare -->

<owl:Class rdf:ID="Doctor">
  <rdfs:subClassOf rdf:resource="&base;Healthcare" />
  <rdfs:comment>This class represents professions of doctor</rdfs:comment>
  <rdfs:label>Doctor</rdfs:label>
</owl:Class>

<owl:Class rdf:ID="Nurse">
  <rdfs:subClassOf rdf:resource="&base;Healthcare" />
  <rdfs:comment>This class represents the nursing profession</rdfs:comment>
  <rdfs:label>Nurse</rdfs:label>
</owl:Class>

<owl:Class rdf:ID="Midwife">
  <rdfs:subClassOf rdf:resource="&base;Healthcare" />
  <rdfs:comment>This class represents the midwifery professions</rdfs:comment>
  <rdfs:label>Midwife</rdfs:label>
</owl:Class>

<!-- Information Services -->

<owl:Class rdf:ID="Archivist">
  <rdfs:subClassOf rdf:resource="&base;Information-Services" />
  <rdfs:comment>This class represents professions relating to the archiving and presevation of information</rdfs:comment>
  <rdfs:label>Archivist</rdfs:label>
</owl:Class>

<owl:Class rdf:ID="Information-Gatherer">
  <rdfs:subClassOf rdf:resource="&base;Information-Services" />
  <rdfs:comment>This class represents professions relating to the gathering of information</rdfs:comment>
  <rdfs:label>Information Gatherer</rdfs:label>
</owl:Class>

<owl:Class rdf:ID="Intelligencer">
  <rdfs:subClassOf rdf:resource="&base;Information-Gatherer" />
  <rdfs:comment>This class represents professions relating to the illicit gathering and processing of information i.e. spy</rdfs:comment>
  <rdfs:label>Intelligencer</rdfs:label>
</owl:Class>

<owl:Class rdf:ID="Researcher">
  <rdfs:subClassOf rdf:resource="&base;Information-Gatherer" />
  <rdfs:comment>This class represents professions relating to research</rdfs:comment>
  <rdfs:label>Researcher</rdfs:label>
</owl:Class>

<owl:Class rdf:ID="Torturer">
  <rdfs:subClassOf rdf:resource="&base;Information-Gatherer" />
  <rdfs:comment>This class represents professions relating to the gathering of informaton through "cruel and unusual" coercion</rdfs:comment>
  <rdfs:label>Torturer</rdfs:label>
</owl:Class>

<!-- Manual -->

<owl:Class rdf:ID="Skilled">
  <rdfs:subClassOf rdf:resource="&base;Manual" />
  <rdfs:comment>This class represents professions relating to skilled manual labour</rdfs:comment>
  <rdfs:label>Manual (Skilled)</rdfs:label>
</owl:Class>

<owl:Class rdf:ID="Unskilled">
  <rdfs:subClassOf rdf:resource="&base;Manual" />
  <rdfs:comment>This class represents professions relating to unskilled manual labour</rdfs:comment>
  <rdfs:label>Manual (Unskilled)</rdfs:label>
</owl:Class>

  <!-- Religious -->

<owl:Class rdf:ID="Martyr">
  <rdfs:subClassOf rdf:resource="&base;Religious" />
  <rdfs:comment>This class represents professions relating to martyrdom</rdfs:comment>
  <rdfs:label>Martyr</rdfs:label>
</owl:Class>

<owl:Class rdf:ID="Saint">
  <rdfs:subClassOf rdf:resource="&base;Religious" />
  <rdfs:comment>This class represents professions relating to sainthood</rdfs:comment>
  <rdfs:label>Saint</rdfs:label>
</owl:Class>

<!-- Medical Properties -->

  <owl:ObjectProperty rdf:ID="specialisation">
    <rdfs:label>Subject</rdfs:label>
    <rdfs:comment>This property specifies a subject</rdfs:comment>
    <rdfs:domain rdf:resource="&base;Healthcare"/>
    <rdfs:range> 
    <owl:Class>
        <owl:unionOf rdf:parseType="Collection">
	    <owl:Class rdf:about="&omb;Mental-Illness"/>
	    <owl:Class rdf:about="&omb;Physical-Illness"/>
	    <owl:Class rdf:about="&omb;Physical-Injury"/>
	    <owl:Class rdf:about="&omb;Emotional-Crisis"/>
        </owl:unionOf>
    </owl:Class>    		
    </rdfs:range> 
  </owl:ObjectProperty> 

<!-- Educational Properties -->

  <owl:ObjectProperty rdf:ID="subject">
    <rdfs:label>Subject</rdfs:label>
    <rdfs:comment>This property specifies a subject</rdfs:comment>
    <rdfs:domain rdf:resource="&base;Education"/>
    <rdfs:range rdf:resource="&ome;Expression"/>
  </owl:ObjectProperty> 


<!-- Trade -->

  <owl:ObjectProperty rdf:ID="product">
    <rdfs:label>Product</rdfs:label>
    <rdfs:comment>This property specifies a product</rdfs:comment>
    <rdfs:domain rdf:resource="&base;Trade"/>
    <rdfs:range> 
    <owl:Class>
        <owl:unionOf rdf:parseType="Collection">
	    <owl:Class rdf:about="&omb;Character"/>
	    <owl:Class rdf:about="&ome;Item"/>
	    <owl:Class rdf:about="&loc;Space"/>
        </owl:unionOf>
    </owl:Class>    		
    </rdfs:range> 
  </owl:ObjectProperty>    

</rdf:RDF>
