<?xml version="1.0"?>
<!DOCTYPE owl [
<!ENTITY ome "http://www.r4isstatic.com/linkeddata/ontologies/ontomedia/core/expression#">
<!ENTITY xprop "http://www.r4isstatic.com/linkeddata/ontologies/ontomedia/ext/common/exprop#">
<!ENTITY dc "http://purl.org/dc/elements/1.1/">
<!ENTITY dct "http://purl.org/dc/terms/">
<!ENTITY xsd "http://www.w3.org/2001/XMLSchema#">
<!ENTITY rdf "http://www.w3.org/1999/02/22-rdf-syntax-ns#">
<!ENTITY owl "http://www.w3.org/2002/07/owl#">
<!ENTITY rdfs "http://www.w3.org/2000/01/rdf-schema#">
<!ENTITY base "http://www.r4isstatic.com/linkeddata/ontologies/ontomedia/ext/events/eventprop#">
]>


<rdf:RDF
 xmlns:ome="&ome;"
 xmlns:xprop="&xprop;"
 xmlns:dc="&dc;"
 xmlns:dct="&dct;"
 xmlns:xsd="&xsd;"
 xmlns:rdf="&rdf;"
 xmlns:owl="&owl;"
 xmlns:rdfs="&rdfs;"
 xml:base="&base;"
>
	 	 

<owl:Ontology rdf:about="&base;">
 <rdfs:label>OntoMedia Trait Representation</rdfs:label>
 <dc:title xml:lang="en">OntoMedia Expression Property Representation</dc:title>
 <dc:description xml:lang="en">OntoMedia (Ontology for Media) has been designed to describe the interactions occurring in multimedia.</dc:description>
 <dc:creator>Michael O. Jewell (mailto:moj@ecs.soton.ac.uk)</dc:creator>
 <dc:creator>K Faith Lawrence (mailto:kf03r@ecs.soton.ac.uk)</dc:creator>
 <dc:creator>Mischa M Tuffield (mailto:mmt04r@ecs.soton.ac.uk)</dc:creator>
 <dct:created>2005-05-11</dct:created>
 <owl:versionInfo>0.2</owl:versionInfo>
</owl:Ontology>

<!-- Event Properties -->

  <owl:Class rdf:ID="Event-Properties">
    <rdfs:label>Event Properties</rdfs:label>
    <rdfs:comment>This class represents additional properties for events</rdfs:comment>
    <!-- <rdfs:subClassOf rdf:resource="&ome;Content" /> -->
  </owl:Class>


<!-- Event Properties Extensions -->

  <owl:Class rdf:ID="Consent-Properties">
    <rdfs:label>Expression Properties</rdfs:label>
    <rdfs:comment>This class represents the consensual nature of the event</rdfs:comment>
    <rdfs:subClassOf rdf:resource="#Event-Properties" />
  </owl:Class>


<!-- Consent Classes -->

  <owl:Class rdf:ID="Consent-Given">
    <rdfs:label>Consent Given</rdfs:label>
    <rdfs:comment>This class represents the concept of consent being given for an action by the subject to the object</rdfs:comment>
    <rdfs:subClassOf rdf:resource="#Consent-Properties" />
    <owl:disjointWith rdf:resource="#Consent-Implied" />
    <owl:disjointWith rdf:resource="#Consent-Not-Given" />
    <owl:disjointWith rdf:resource="#Consent-Unclear" />   
  </owl:Class>
  
  <owl:Class rdf:ID="Consent-Implied">
    <rdfs:label>Consent Implied</rdfs:label>
    <rdfs:comment>This class represents the concept of consent being implied for an action by the subject to the object</rdfs:comment>
    <rdfs:subClassOf rdf:resource="#Consent-Properties" />
    <owl:disjointWith rdf:resource="#Consent-Given" />
    <owl:disjointWith rdf:resource="#Consent-Not-Given" />
    <owl:disjointWith rdf:resource="#Consent-Unclear" />
  </owl:Class>
  
  <owl:Class rdf:ID="Consent-Not-Given">
    <rdfs:label>Consent Not Given</rdfs:label>
    <rdfs:comment>This class represents the concept of consent not being given for an action by the subject to the object</rdfs:comment>
    <rdfs:subClassOf rdf:resource="#Consent-Properties" />
    <owl:disjointWith rdf:resource="#Consent-Given" />
    <owl:disjointWith rdf:resource="#Consent-Implied" />
    <owl:disjointWith rdf:resource="#Consent-Unclear" />
  </owl:Class>
  
  <owl:Class rdf:ID="Consent-Unclear">
    <rdfs:label>Expression Properties</rdfs:label>
    <rdfs:comment>This class represents the concept of consent being unclear for an action by the subject to the object</rdfs:comment>
    <rdfs:subClassOf rdf:resource="#Consent-Properties" />
    <owl:disjointWith rdf:resource="#Consent-Given" />
    <owl:disjointWith rdf:resource="#Consent-Implied" />
    <owl:disjointWith rdf:resource="#Consent-Not-Given" />
  </owl:Class>     

<!-- Transformation Properties - NOW IN EXPRESSION

  <owl:ObjectProperty rdf:ID="From">
    <rdfs:label>From</rdfs:label>
    <rdfs:comment>This property specifies the starting entity of the transformation</rdfs:comment>
    <rdfs:domain rdf:resource="&ome;Transformation"/>
    <rdfs:range rdf:resource="&ome;Entity"/>
  </owl:ObjectProperty> 
  
  <owl:ObjectProperty rdf:ID="To">
    <rdfs:label>To</rdfs:label>
    <rdfs:comment>This property specifies the final entity of the transformation</rdfs:comment>
    <rdfs:domain rdf:resource="&ome;Transformation"/>
    <rdfs:range rdf:resource="&ome;Entity"/>
  </owl:ObjectProperty> 
-->
  
</rdf:RDF>  
  
